\section{UNDERSTANDING THE HOLDER INEUQALITY}

\begin{enumerate}
	\item \textbf{Solution:}
	\begin{enumerate}
		\item Since the $\ln x$ is a concave function, by the Jensen's inequality
		$$\lambda \ln\alpha +(1-\lambda)\ln \beta\le \ln(\lambda \alpha+(1-\lambda)\beta)$$
		Take the exponential of each side, we complete the proof
		$$\alpha^\lambda\beta^{1-\lambda}\le \lambda\alpha+(1-\lambda)\beta$$
		Q.E.D.
		\item Apply the inequality of part(a), we obtain
		\begin{align*}
		\sum_{i=1}^{n}|\hat{x}_i\hat{y}_i|&=\sum_{i=1}^{n}|\frac{x_i}{\left\|x\right\|_p}\cdot \frac{y_i}{	\left\|y\right\|_q}|\\
		&=\sum_{i=1}^{n} |\frac{(x_i^p)^{\frac{1}{p}}}{\sum_{i=1}^{n}(|x|^p)^{\frac{1}{p}}}\cdot \frac{(y_i^q)^{\frac{1}{q}}}{\sum_{i=1}^{n}(|y|^q)^{\frac{1}{q}}}|\\
		&\le \frac{1}{p} \sum_{i=1}^{n}\frac{|x_i|^p}{\sum_{i=1}^{n}|x|^p} + \frac{1}{q}\frac{|y_i|^q}{\sum_{i=1}^{n}|y|^q}\\
		&=\frac{1}{p} \sum_{i=1}^{n} |\hat{x}_i|^p+\frac{1}{q} \sum_{i=1}^{n} |\hat{y}_i|^q\\
		&=1
		\end{align*}
		Q.E.D.
		\item With the above results
		\begin{align*}
		\sum_{i=1}^{n}|\hat{x}_i\hat{y}_i| =\sum_{i=1}^{n} |\frac{(x_i^p)^{\frac{1}{p}}}{\sum_{i=1}^{n}(|x|^p)^{\frac{1}{p}}}&\cdot \frac{(y_i^q)^{\frac{1}{q}}}{\sum_{i=1}^{n}(|y|^q)^{\frac{1}{q}}}|\le 1\\
		\Leftrightarrow  \frac{\sum_{i=1}^{n}|\hat{x}_i\hat{y}_i|}{\sum_{i=1}^{n}(|x|^p)^{\frac{1}{p}} \cdot \sum_{i=1}^{n}(|y|^q)^{\frac{1}{q}}}&\le 1\\
		\Leftrightarrow \frac{|x^Ty|}{\left\|x\right\|_p,\left\|y\right\|_q}&\le 1\\
		\Leftrightarrow |x^Ty|&\le \left\|x\right\|_p\left\|y\right\|_q
		\end{align*}
		Q.E.D.
		\item 
		\begin{align*}
		(||x||_p)^p&=\sum_{i=1}^n (x_i+y_i)^p\\
		&=\sum_{i=1}^nx_i(x_i+y_i)^{p-1} + \sum_{i=1}^n y_i(x_i+y_i)^{q-1}\\
		&\le (\sum_{i=1}^nx_i^p)^{\frac{1}{p}}(\sum_{i=1}^n(x_i+y_i)^{(p-1)q})^\frac{1}{q} + (\sum_{i=1}^ny_i^p)^{\frac{1}{q}}(\sum_{i=1}^n(x_i+y_i)^{(p-1)q})^\frac{1}{q}\\
		&=(||x||_p+||y||_p)(\sum_{i=1}^n(x_i+y_i)^p)^{1-\frac{1}{p}}
		\end{align*}
		This implies that
		\begin{align*}
		(\sum_{i=1}^n(x_i+y_i)^p)^{1-1+\frac{1}{p}} \le||x||_p+||y||_p\\
		\Leftrightarrow ||x+y||_p\le||x||_p+||y||_p
		\end{align*}
		Q.E.D.
	\end{enumerate}
\end{enumerate}